Add simple example with two locations

src/examples/simple.v
@@ -8,8 +8,7 @@ From self.lang Require Import notation lang.
 From self.algebra Require Import view.
 From self.base Require Import primitive_laws class_instances.
 From self.high Require Import proofmode.
-From self.high Require Import dprop.
-From self Require Import weakestpre.
+From self.high Require Import dprop weakestpre recovery_weakestpre.
 
 Definition prog : expr := let: "l" := ref #1 in ! "l".
 
@@ -19,7 +18,7 @@ Definition pure : expr :=
   "a" + "b".
 
 Section specs.
-  Context `{!nvmBaseG Σ, !nvmG Σ}.
+  Context `{!nvmG Σ}.
 
   Lemma wp_bin_op : ⊢ WP (#1 + #2) {{ v, ⌜1 = 1⌝ }}.
   Proof.
@@ -41,6 +40,26 @@ Section specs.
 End specs.
 
 Section simple_increment.
-  Context `{!nvmBaseG Σ}.
+  Context `{!nvmG Σ}.
+
+  Definition incr (ℓa ℓb : loc) : expr :=
+    #ℓa <- #1 ;;
+    WB #ℓa ;;
+    Fence ;;
+    #ℓb <- #1.
+
+  Definition recover (ℓa ℓb : loc) : expr :=
+    let: "a" := ! #ℓa in
+    let: "b" := ! #ℓb in
+    if: "b" ≤ "a"
+    then #() #() (* Get stuck. *)
+    else #().
+
+  Lemma wpc_incr (ℓa ℓb : loc) : expr :=
+
+  Lemma incr_safe s k E ℓa ℓb :
+    ⊢ wpr s k E (incr ℓa ℓb) (recover ℓa ℓb) (λ _, True%I) (λ _ _, True%I).
+  Proof.
+  Abort.
 
 End simple_increment.
